Veir/Dialects/Arith/OpInfo.lean
@@ -164,7 +164,7 @@ def OperationPtr.verifyArithExtendedOp {OpInfo : Type} [HasOpInfo OpInfo]
     (op : OperationPtr) (ctx : WfIRContext OpInfo)
     (opIn : op.InBounds ctx.raw) (secondResultIsI1 : Bool) : Except String PUnit := do
   op.verifyPlainOpCounts ctx opIn 2 2
-  let instrName := String.fromUTF8! (HasOpInfo.name (op.getOpType ctx.raw opIn))
+  let instrName := String.fromUTF8! (IsOpCode.name (op.getOpType ctx.raw opIn))
   ((op.getOperand! ctx.raw 0).getType! ctx.raw).verifyIntegerType
     s!"{instrName}: Expected operand 0 to have integer type"
   ((op.getOperand! ctx.raw 1).getType! ctx.raw).verifyIntegerType
